arch/msp430/machine.s.dfy
@@ -1,0 +1,175 @@
+include "../../lib/bv16_ops.dfy"
+include "flat.s.dfy"
+// include "../../lib/bv20_ops.dfy"
+
+module rv_machine {
+    import opened integers
+    import opened bv16_ops
+    // import bv20_ops
+    import opened flat
+
+    /* registers definitions */
+
+    datatype reg_t =  
+        // | PC
+        | SP
+        // | R2
+        | R3
+        | R4
+        | R5
+        | R6
+        | R7
+        | R8
+        | R9
+        | R10
+        | R11
+        | R12
+        | R13
+        | R14
+        | R15
+
+    /* state definition */
+
+    type regs_t = map<reg_t, uint20>
+
+    function method truncate_20_to_16(v: uint20): uint16
+    {
+        v % BASE_16
+    }
+
+    datatype operand_t = 
+        | Reg(r: reg_t)
+        | Idx(r: reg_t, index: uint16)
+        | RegIndir(r: reg_t, inc: bool)
+        | Imm(i: uint16)
+    
+    datatype state = state(
+        regs: regs_t,
+        flat: flat_t,
+        ok: bool)
+    {
+        function read_reg16(r: reg_t): uint16
+        {
+            if r in regs then truncate_20_to_16(regs[r]) else 0
+        }
+
+        // will overrite higher bits
+        function write_reg16(r: reg_t, value: uint16): state
+        {
+            this.(regs := this.regs[r := value])
+        }
+
+        function write_reg20(r: reg_t, value: uint20): state
+        {
+            this.(regs := this.regs[r := value])
+        }
+    }
+
+    function eval_operand(s: state, op: operand_t): uint16
+        // requires op.Reg? || op.Imm?
+    {
+        match op
+            case Reg(r) => s.read_reg16(r)
+            case Imm(i) => i
+            case _ => 0
+    }
+
+    predicate valid_state(s: state)
+    {
+        s.ok
+    }
+
+    datatype ins_t = 
+        | MSP_ADD_W(src: operand_t, dst: operand_t)
+        | MSP_ADDC_W(src: operand_t, dst: operand_t)
+        | MSP_SUB_W(src: operand_t, dst: operand_t)
+        | MSP_MOV_W(src: operand_t, dst: operand_t)
+        | MSP_MOV_B(src: operand_t, dst: operand_t)
+        | MSP_CMP_W(src: operand_t, dst: operand_t)
+        | MSP_RRAX_W(dst: operand_t)
+        | MSP_PUSHM_W(dst: operand_t, n: operand_t)
+        | MSP_POPM_W(dst: operand_t, n: operand_t)
+        // BR
+        // RET
+        // CALL
+
+    predicate eval_ins(ins: ins_t, s: state, r: state)
+    {
+        if !s.ok then
+            !r.ok
+        else
+            r.ok && (valid_state(s) ==> valid_state(r))
+    }
+
+    /* control flow definitions */
+
+    datatype cond =
+        | Eq(o1: operand_t, o2: operand_t)
+        | Ne(o1: operand_t, o2: operand_t)
+        | LO(o1: operand_t, o2: operand_t) // Jump if lower (unsigned)
+        | HS(o1: operand_t, o2: operand_t) // Jump if higher or same (unsigned)
+    
+    datatype code =
+        | Ins(ins: ins_t)
+        | Block(block: codes)
+        | While(whileCond: cond, whileBody: code)
+        | IfElse(ifCond: cond, ifTrue: code, ifFalse: code)
+        | Function(name: string, functionBody: codes)
+        | Comment(com: string)
+
+    datatype codes =
+      | CNil
+      | va_CCons(hd: code, tl: codes)
+
+    predicate eval_block(block: codes, s: state, r: state)
+    {
+        if block.CNil? then
+            r == s
+        else
+            exists r': state :: eval_code(block.hd, s, r') && eval_block(block.tl, r', r)
+    }
+
+    function eval_cond(s: state, c: cond):bool
+    {
+        match c
+          case Eq(o1, o2)  => (eval_operand(s, o1) == eval_operand(s, o2))
+          case Ne(o1, o2)  => (eval_operand(s, o1) != eval_operand(s, o2))
+          case LO(o1, o2)  => (eval_operand(s, o1) < eval_operand(s, o2))
+          case HS(o1, o2)  => (eval_operand(s, o1) >= eval_operand(s, o2))
+    }
+
+    predicate eval_if_else(cond:cond, ifT:code, ifF:code, s:state, r:state)
+        decreases if eval_cond(s, cond) then ifT else ifF
+    {
+        if s.ok then
+            (if eval_cond(s, cond) then eval_code(ifT, s, r) else eval_code(ifF, s, r))
+        else
+            !r.ok
+    }
+
+    predicate eval_while(condition:cond, body:code, n: nat, s: state, r: state)
+        decreases body, n
+    {
+        if s.ok then
+            if n == 0 then
+                !eval_cond(s, condition) && (s == r)
+            else
+              exists s': state :: eval_cond(s, condition)
+                      && eval_code(body, s, s')
+                      && eval_while(condition, body, n - 1, s', r)
+        else
+            !r.ok
+    }
+
+    predicate eval_code(c: code, s: state, r: state)
+        decreases c, 0
+    {
+        match c
+            case Ins(ins) => eval_ins(ins, s, r)
+            case Block(block) => eval_block(block, s, r)
+            case While(condition, body) => exists n:nat :: eval_while(condition, body, n, s, r)
+            case Function(name, body) => eval_block(body, s, r)
+            case IfElse(cond, ifT, ifF) => eval_if_else(cond, ifT, ifF, s, r)
+            case Comment(com) => s == r
+    }
+}
