lib/generic_bv_ops.dfy
@@ -28,6 +28,7 @@ module integers
     type uint10  = i :int | 0 <= i < 1024
     type uint12  = i :int | 0 <= i < 4096
     type uint16  = i :int | 0 <= i < BASE_16
+    type uint20  = i :int | 0 <= i < 1048576
     type uint32  = i :int | 0 <= i < BASE_32
     type uint64  = i :int | 0 <= i < BASE_64
     type uint128 = i :int | 0 <= i < BASE_128
